remove commented code

IMP.lean
@@ -13,17 +13,6 @@ inductive sinstr : Type
 | SMult
 
 def total_map (A : Type) := string -> A
-/--/
-def t_empty {A : Type} (v : A) : total_map A :=
-  (fun _ : v).
-
-def partial_map (A : Type) := total_map (option A)
-
-def update {A : Type} (m : partial_map A)
-           (x : string) (v : A) :=
-  (x !-> Some v ; m).
-
-def empty_st := (_ !-> 0) -/
 
 def st := total_map nat
 
@@ -52,42 +41,6 @@ def s_execute : st -> (list nat) -> (list sinstr) -> (list nat)
                                       | _ := s_execute state stack prog
                                       end
 
-/-
-def s_execute : st -> (list nat) -> (list sinstr) -> (list nat)
-  | state stack list.nil := stack
-  | state stack (h::t) := match h with
-                            | sinstr.SPush n := s_execute state (n::stack) t
-                            | sinstr.SLoad x := s_execute state ((state x)::stack) t
-                            | sinstr.SPlus := match stack with
-                                              | h1::h2::stack_tail := s_execute state ((h2 + h1)::stack_tail) t 
-                                              | _ := s_execute state stack t
-                                              end
-                            | sinstr.SMinus := match stack with
-                                              | h1::h2::stack_tail := s_execute state ((h2 - h1)::stack_tail) t 
-                                              | _ := s_execute state stack t
-                                                end
-                            | sinstr.SMult := match stack with
-                                                | h1::h2::stack_tail := s_execute state ((h2 * h1)::stack_tail) t 
-                                                | _ := s_execute state stack t
-                                                end
-                         end-/
-
-/-
-def s_execute : st -> (list nat) -> (list sinstr) -> (list nat)
-| state stack list.nil := stack
-| state stack ((sinstr.SPush n)::prog) := s_execute state (n::stack) prog
-| state stack ((sinstr.SLoad x)::prog) := s_execute state ((state x)::stack) prog
-| state (h1::h2::stack_tail) (sinstr.SPlus::prog) := s_execute state ((h2 + h1)::stack_tail) prog
-| state (h1::h2::stack_tail) (sinstr.SMinus::prog) := s_execute state ((h2 - h1)::stack_tail) prog                                 
-| state (h1::h2::stack_tail) (sinstr.SMult::prog) := s_execute state ((h2 * h1)::stack_tail) prog
-| state stack (_::prog) := s_execute state stack prog
--/
-
-/-
-example (empty_st : st)  :  (s_execute empty_st [] [sinstr.SPush 5, sinstr.SPush 3, sinstr.SPush 1, sinstr.SMinus]) 
-    = [2, 5] :=
--/
-
 def s_compile : aexp -> (list sinstr)
   | (aexp.ANum n) := [sinstr.SPush n]
   | (aexp.AId x) := [sinstr.SLoad x]                         
@@ -95,53 +48,55 @@ def s_compile : aexp -> (list sinstr)
   | (aexp.AMinus a1 a2)  := s_compile a1 ++ s_compile a2 ++ [sinstr.SMinus]
   | (aexp.AMult a1 a2) := s_compile a1 ++ s_compile a2 ++ [sinstr.SMult]
 
+/- Expanded version -/
 lemma s_compile_correct_prog : forall (state : st) (prog1 : list sinstr) (prog2 : list sinstr) (stack : list nat),
     s_execute state stack (prog1 ++ prog2) = s_execute state (s_execute state stack prog1) prog2 :=
 begin
   intros state prog1 prog2,
   induction prog1,
-  case list.nil { intro stack, simp, rw [s_execute] },
+  case list.nil { intro stack, simp [s_execute] },
   case list.cons { intro stack, induction prog1_hd,
-    case sinstr.SPush { simp, repeat { rw[s_execute] }, intros, destruct stack; rw prog1_ih; intros; refl},
-    case sinstr.SLoad { simp, repeat { rw[s_execute] }, intros, destruct stack; rw prog1_ih; intros; refl},
-    case sinstr.SPlus { simp, repeat { rw[s_execute] }, intros, cases stack, 
+    case sinstr.SPush { simp [s_execute], intros, destruct stack; rw prog1_ih; intros; refl},
+    case sinstr.SLoad { simp [s_execute], intros, destruct stack; rw prog1_ih; intros; refl},
+    case sinstr.SPlus { simp [s_execute], intros, cases stack, 
       case list.nil { rw prog1_ih, refl },
       case list.cons { cases stack_tl,
         case list.nil { rw prog1_ih, refl },
-        case list.cons { repeat { rw[s_execute] }, rw prog1_ih }  
+        case list.cons { simp [s_execute], rw prog1_ih }  
       }
     },
-    case sinstr.SMinus { simp, repeat { rw[s_execute] }, intros, cases stack, 
+    case sinstr.SMinus { simp [s_execute], intros, cases stack, 
       case list.nil { rw prog1_ih, refl },
       case list.cons { cases stack_tl,
         case list.nil { rw prog1_ih, refl },
-        case list.cons { repeat { rw[s_execute] }, rw prog1_ih }  
+        case list.cons { simp [s_execute], rw prog1_ih }  
       }
     },
-    case sinstr.SMult { simp, repeat { rw[s_execute] }, intros, cases stack, 
+    case sinstr.SMult { simp [s_execute], intros, cases stack, 
       case list.nil { rw prog1_ih, refl },
       case list.cons { cases stack_tl,
         case list.nil { rw prog1_ih, refl },
-        case list.cons { repeat { rw[s_execute] }, rw prog1_ih }  
+        case list.cons { simp [s_execute], rw prog1_ih }  
       }
     }
   }
 end
 
+/- Condensed Version -/
 lemma s_compile_correct_prog' : forall (state : st) (prog1 : list sinstr) (prog2 : list sinstr) (stack : list nat),
     s_execute state stack (prog1 ++ prog2) = s_execute state (s_execute state stack prog1) prog2 :=
 begin
   intros state prog1 prog2,
   induction prog1,
-  case list.nil { intro stack, simp, rw [s_execute] },
+  case list.nil { intro stack, simp [s_execute] },
   case list.cons { intro stack; induction prog1_hd;
-    simp; repeat { rw[s_execute] }; intros;
+    simp [s_execute]; intros;
     try { destruct stack; rw prog1_ih; intros; refl };
     try { cases stack, 
       case list.nil { rw prog1_ih, refl },
       case list.cons { cases stack_tl,
         case list.nil { rw prog1_ih, refl },
-        case list.cons { repeat { rw[s_execute] }, rw prog1_ih }  
+        case list.cons { simp [s_execute], rw prog1_ih }  
       } 
     }
   }
@@ -153,11 +108,10 @@ lemma s_compile_correct_general (state : st) (e : aexp) : forall (stack : list n
 begin
   induction e;
   intro stack;
-  try { refl }; intros; rw [aeval]; rw [s_compile];
-  repeat { rw s_compile_correct_prog };
-  rw [e_ih_a1];
-  rw [e_ih_a2]; 
-  repeat { rw [s_execute] };
+  try { refl }; intros; simp [aeval, s_compile];
+  repeat { rw s_compile_correct_prog' };
+  rw [e_ih_a1, e_ih_a2]; 
+  simp [s_execute];
   refl
 end
 
